\documentclass[11pt]{article}
\input{/Users/markwang/.preamble}
\begin{document}



\begin{align*}
    Max &\quad \sum_{(s,u)\in E} f_{sv} - \sum_{(v,s)\in\E} f_{vs} 
    & 
    Max &\quad d^T f \\
    st. &\sum_{(v,u)\in E} f_{vu} - \sum_{(u,v) \in E} f_{uv} = 0 \qquad \forall u\in V \setminus \{s,t\} 
    & 
    s.t. &\quad Af \geq b \quad Af \leq b \\
    &0 \leq f_e \leq c_e \qquad \forall e\in E 
    & 
    & f_e \geq 0
    \\
\end{align*}
where
\[
    \underset{m\times 1}{d} 
    \qquad 
    \underset{(n-2+m)\times m}{A} = 
    \begin{pmatrix}
        \underset{(n-2)\times m}{B} \\
        I_m \\ 
    \end{pmatrix} 
    \qquad 
    \underset{(n-2+m)\times 1}{b} = 
    \begin{pmatrix}
        \underset{(n-2)\times 1}{0} \\
        C \\ 
    \end{pmatrix}
\]


\[
    d_{uv} = 
    \begin{cases}
        1  & u = s \quad (s,v)\in E  \\ 
        -1 & v = s \quad (u,s)\in E  \\ 
        0 & otherwise
    \end{cases}  
    \qquad 
    \qquad 
    B_{ve} = 
    \begin{cases}
        1 & (\cdot , v) = e \\
        -1 & (v, \cdot ) = e \\ 
        0 & otherwise \\
    \end{cases}    
\]

\noindent Let $|E| = m$ and $|v| = n$. PLP has $m$ variables and $2(n-2)+m$ varialbes. Supposedly, the dual has $2(n-2) + m$ variables and $m$ constraints. However, we can reduce number of dual variables to $n-2+m$ by noticing that 
\[
    Ax = b \iff Ax \leq b \quad (-A) x \leq (-b) \iff 
    \tilde{A}x =
    \begin{pmatrix}
        A \\
        -A
    \end{pmatrix}
    x \leq 
    \begin{pmatrix}
        b \\
        -b \\
    \end{pmatrix}
    =  \tilde{b}
\]
Given dual varaibles $y = \begin{pmatrix} y_1 & y_2 \end{pmatrix} \in\R^{2m}$ where $y_1,y_2\in\R^{m+}$ have the following dual constraints 
\[
    \tilde{A}^T y = 
    \begin{pmatrix}
        A^T & -A^T 
    \end{pmatrix}
    \begin{pmatrix}
        y_1 \\
        y_2 \\ 
    \end{pmatrix} 
    = A^T(y_1 - y_2) 
    = A^T y'
    \geq c 
\]
for some $y' = y_1 - y_2 \in\R^m$. Note we reduce number of dual variables by half, i.e. non-negative $y_1,y_2 \in\R^{m+}$ to $y' \in\R^m$, which can be negative

\begin{align*}
    Min &\sum_{e\in E} c_e y_e 
    &
    Min \quad &b^T \tilde{y}
    = b^T \begin{pmatrix}
        x \\ y \\
    \end{pmatrix}
    \\
    s.t.& \quad x_v - x_u + y_{uv} \geq 0 \qquad \forall (u,v)\in E 
    & 
    s.t.& A^T \tilde{y} \geq d \\
    & x_s = 1 \quad x_t = 0  
    &
    &y \geq 0 
    \\
    & y_e \geq 0 \qquad \forall e\in E
\end{align*}
where $\underset{(n-2)\times 1}{x}$ has one value for each $V\setminus \{s,t\}$, and $\underset{m\times 1}{y}$ has one value for each $e\in E$


\[
    b^T \tilde{y} = 
    \begin{pmatrix}
        \underset{(n-2)\times 1}{0} & C \\
    \end{pmatrix}
    \begin{pmatrix}
        \underset{(n-2)\times 1} x \\
        \underset{m\times 1} y \\ 
    \end{pmatrix}
    = \sum_{e\in E} c_e y_e   
    \qquad \text{and}\qquad 
    y\geq 0 \quad \rightarrow \quad y_e \geq 0 \forall e\in E
\]

\[
    A^T \tilde{y} = 
    \begin{pmatrix}
        \underset{m\times (n-2)}{B^T} & I_m \\ 
    \end{pmatrix}    
    \begin{pmatrix}
        x \\ y \\ 
    \end{pmatrix}
    = 
    B^T x  + I_m y 
    \qquad 
    (I_m y)_{e} = y_e
\]
\[
    (B^T)_{ev} = B_{ve} = 
    \begin{cases}
        1 & (\cdot , v) = e \\
        -1 & (v, \cdot ) = e \\ 
        0 & otherwise \\
    \end{cases}   
    \quad 
    \rightarrow 
    \quad 
    (B^T x)_{e=(v_1,v_2)} = \sum_{v\in V\setminus \{s,t\}} (B^T)_{ev} x_v = B_{v_1 e} x_{v_1} + B_{v_2 e} x_{v_2} = x_{v_1} - x_{v_2}
\]


therefore for edges whose vertices consists of neither $s$ nor $t$
\[
    A^T \tilde{y} \geq d 
    \quad \rightarrow \quad 
    x_v - x_u + y_{uv} \geq 0 \quad \forall (u,v)\in E: u,v\neq s,t
\]
For edges that connects $s$, we have 
\[
    x_u + y_{su} \geq 1 
    \quad 
    x_s + y_{us} \geq -1
\]
if we set variables $x_s=1$, then we can write above as 
\[
    x_u - x_s + y_{su} \geq 0 
    \quad 
    x_s - x_u + y_{us} \geq 0   
\]
to fit with how the above formulation. Setting $x_t=0$ does the trick for edges that connects $t$







\end{document}
